Bool.v
@@ -1,0 +1,105 @@
+Require Import Metalib.Metatheory.
+From STLCZK Require Import Stlc.
+From STLCZK Require Import Gadgets.
+From STLCZK Require Import R1cs.
+From STLCZK Require Import GaloisField.
+From STLCZK Require Import Ltac.
+
+Require Import Coqprime.elliptic.ZEll.
+Require Import Coq.Numbers.BinNums.
+Require Import Coqprime.elliptic.GZnZ.
+Require Import Coq.ZArith.Znumtheory.
+Require Import Coq.ZArith.BinIntDef.
+Import Z.
+Require Import Coq.ZArith.BinInt.
+Require Import Coq.Vectors.VectorDef.
+
+From Coq Require Import Ring.
+From Coq Require Import Field.
+Require Import Coq.micromega.Lia.
+
+Module BoolGadget(PF: GaloisField).
+  Import PF.
+  Include Gadget PF.
+  Import VectorNotations.
+
+  (** Example 1: Division *)
+  Definition andbg :=
+    <{ \_: Bool * Bool,
+           (fst #0) && (snd #0) }>. 
+
+  Definition andg_check :=
+    <[ { (1i[0]) * (1i[1]) == (1o[0]) } ]>.  
+
+  Ltac deconj :=
+    repeat match goal with
+    | [H: _ /\ _ |- _ ] => invert H
+    end.
+
+  Ltac pksimpl :=
+    repeat match goal with
+           |[H: _ |- context[pkmul ?a 0:%p]] => rewrite Rmul_zero_l
+           |[H: _ |- context[pkmul 1:%p ?a]] => rewrite (Rmul_1_l (F_R FTH))
+           |[H: _ |- context[pkmul 0:%p ?a]] =>
+            replace (pkmul 0:%p a) with (pkmul a 0:%p) by (apply (Rmul_comm (F_R FTH)))
+           |[H: _ |- pksub 0:%p ?a = 0:%p] =>
+            apply Rsub_0_0
+           end.
+  
+  (** Second equivalence proof over r1cs *)
+  Theorem and_equiv_r1cs:
+    andbg <=*=> andg_check.
+  Proof.    
+    unfold r1cs_lambda_tequiv, andbg, andg_check.
+    intros args results inps outs vars t t' HTe Hins Houts.
+    cbn in vars.
+
+    unfold cannonical in Hins, Houts;
+    unfold correct, correct_lt;
+    split; intros HPrem;      
+      pose proof (vec2_proj inps); pose proof (vec1_proj outs);exists_inverter; deconj; subst.
+    invert HTe.
+    cbn in H7.
+    
+    pose proof (inversion_principle_bool_bool args a0 b H0 H5); invert H3.
+    - deconj. pose proof (inversion_principle_bool results a H H2).
+    (** Invert inps *)
+    invert HTe; invert H. invert H5. invert H2; invert H5; pksimpl.
+    - cbn in H7.
+      pose proof (vec1_proj v); exists_inverter; subst.
+      destruct (inversion_principle_bool e2 a H10 H2).
+      destruct H.
+      subst.
+      econstructor; cbn; pksimpl.
+      deconj.
+      econstructor; cbn; pksimpl.
+      solve_stlc.
+    invert H.
+    invert H9.
+    
+    - repeat match goal with
+             |[H: Vfp 1 |- _] => pose proof (vec1_proj H); exists_inverter; subst; clear H
+             |[H: Vfp 2 |- _] => pose proof (vec2_proj H); exists_inverter; subst; clear H
+             |[H: exp_typ _ _ _ |- _] => invert H
+             |[H: _ \/ _ |- _ ]=> invert H
+             end; try solve[invert HTe];
+      econstructor; cbn;
+        repeat match goal with
+               |[H: _ |- context[pkmul ?a 0:%p]] => rewrite Rmul_zero_l
+               |[H: _ |- context[pkmul 1:%p ?a]] => rewrite (Rmul_1_l (F_R FTH))
+               |[H: _ |- context[pkmul 0:%p ?a]] =>
+                replace (pkmul 0:%p a) with (pkmul a 0:%p) by (apply (Rmul_comm (F_R FTH)))
+               |[H: _ |- pksub 0:%p ?a = 0:%p] =>
+                apply Rsub_0_0
+               end.
+      
+      invert HTargs.
+
+
+      
+      invert HTargs.
+      induction HTa
+      
+  Admitted.
+
+End BoolGadget.     
